WF1, WF2, WF4, and HTREE updates

AppendixE.v
@@ -85,7 +85,15 @@ Definition active_enclave_update (state: enclave_state) (id: enclave_ID): valida
   end.
 
 (* Enclave Elimination *)
-Definition enclave_elimination (state: enclave_state) (id: raw_enclave_ID): enclave_state :=
+Definition enclave_elimination (state: enclave_state) (id: raw_enclave_ID): validatable_enclave_state :=
   match state with
-  | enclave_state_value e memory_range => enclave_state_value e (NatMap.remove id memory_range)
+  | enclave_state_value e memory_range =>
+    match e with
+    | enclave_ID_inactive => enclave_state_valid (enclave_state_value e (NatMap.remove id memory_range))
+    | enclave_ID_active e_raw =>
+      match (eqb id e_raw) with
+      | true => enclave_state_error
+      | false => enclave_state_valid (enclave_state_value e (NatMap.remove id memory_range))
+      end
+    end
   end.
