WellFormed2.v
@@ -1,0 +1,317 @@
+From Coq Require Import Lists.List.
+From Coq Require Import Bool.Bool.
+From Coq Require Import Lia.
+From Coq Require Import FSets.FMapList.
+From Coq Require Import FSets.FMapFacts.
+From Coq Require Import Init.Nat.
+From Coq Require Import Structures.OrderedTypeEx.
+Require Import RuntimeDefinitions.
+Require Import AppendixD.
+Require Import AppendixC.
+Require Import AppendixF.
+Require Import AppendixE.
+Require Import Semantics.
+Require Import MLCOperations.
+Require Import WellFormed.
+
+Module NatMapFacts := NatMapProperties.F.
+Module CacheletMapFacts := CacheletMapProperties.F.
+
+Definition wf4 (sigma: runtime_state): Prop :=
+  forall k mu rho pi p l q e E,
+  (sigma = runtime_state_value k mu rho pi) ->
+  (NatMap.find p pi = Some (process_value (enclave_state_value e E) l q)) ->
+  (e = enclave_ID_inactive \/ (exists raw_e, e = enclave_ID_active raw_e /\ NatMap.In raw_e E)).
+
+Lemma wf4_active_enclave_update : forall e E e' E' r,
+  active_enclave_update (enclave_state_value e E) r = 
+  enclave_state_valid (enclave_state_value e' E') ->
+  (e = enclave_ID_inactive \/ (exists raw_e, e = enclave_ID_active raw_e /\ NatMap.In raw_e E)) ->
+  (e' = enclave_ID_inactive \/ (exists raw_e', e' = enclave_ID_active raw_e' /\ NatMap.In raw_e' E')).
+Proof.
+  intros.
+  destruct r.
+  unfold active_enclave_update in H.
+  case_eq (NatMap.find r E). intros. assert (A1 := H1).
+  destruct (NatMap.find r E) in A1, H.
+  injection A1; injection H; intros; subst; clear A1.
+  right. eexists r. split.
+  reflexivity.
+  assert (NatMap.find r E' <> None).
+  intros contra. rewrite -> H1 in contra. discriminate.
+  apply NatMapFacts.in_find_iff in H2. exact H2.
+  discriminate.
+  intros; destruct (NatMap.find r E).
+  discriminate.
+  discriminate.
+  unfold active_enclave_update in H.
+  injection H; intros; subst.
+  left; reflexivity.
+Qed.
+
+Lemma wf4_enclave_creation : forall e E e' E' mu n x y,
+  enclave_creation (enclave_state_value e E) mu n x y = enclave_state_valid (enclave_state_value e' E') ->
+  (e = enclave_ID_inactive \/ (exists raw_e, e = enclave_ID_active raw_e /\ NatMap.In raw_e E)) ->
+  (e' = enclave_ID_inactive \/ (exists raw_e', e' = enclave_ID_active raw_e' /\ NatMap.In raw_e' E')).
+Proof.
+  intros.
+  unfold enclave_creation in H.
+  destruct x.
+  case_eq (NatMap.find b mu). intros.
+  assert (A0 := H1). destruct (NatMap.find b mu) in A0 , H.
+  case_eq (is_all_zeroes mu b d (length (NatMapProperties.to_list d1)) y).
+  intros. assert (DIS := H2).
+  destruct (is_all_zeroes mu b d (length (NatMapProperties.to_list d1)) y) in DIS, H.
+  unfold add_new_enclave_to_enclave_state in H.
+  case_eq (NatMap.find n E). intros.
+  assert (A1 := H3). destruct (NatMap.find n E) in A1, H.
+  discriminate.
+  discriminate.
+  intros; destruct (NatMap.find n E).
+  discriminate.
+  injection A0; injection H; intros; subst; clear A0.
+  destruct H0.
+  left; exact H0.
+  destruct H0. right.
+  eexists x.
+  destruct H0; split. exact H0.
+  case_eq (eqb n x).
+  intros; apply cmp_to_eq in H5; subst.
+  apply NatMapFacts.add_in_iff; left; reflexivity.
+  intros; apply cmp_to_uneq in H5.
+  apply NatMapFacts.add_in_iff; right; exact H4.
+  discriminate.
+  intros; destruct (is_all_zeroes mu b d (length (NatMapProperties.to_list d1)) y).
+  discriminate.
+  discriminate.
+  discriminate.
+  intros; destruct (NatMap.find b mu).
+  discriminate.
+  discriminate.
+Qed.
+
+Lemma wf4_enclave_elimination : forall e E e' E' r,
+  ((enclave_elimination (enclave_state_value e E) r) = enclave_state_value e' E') ->
+  (exists raw_e, e = enclave_ID_active raw_e /\ NatMap.In raw_e E) ->
+  (exists raw_e', e' = enclave_ID_active raw_e' /\ NatMap.In raw_e' E').
+Proof.
+  intros.
+  destruct e'.
+  unfold enclave_elimination in H.
+  injection H; intros; subst.
+  destruct H0.
+  destruct H0.
+  case_eq (eqb r x).
+  intros; apply cmp_to_eq in H2; subst.
+  eexists x. split. injection H0; intros; subst; reflexivity.
+  (* this case is actually not possible *)
+  give_up.
+  intros; apply cmp_to_uneq in H2.
+  injection H0; intros; subst.
+  destruct H0.
+  eexists x. split. reflexivity.
+  apply NatMapFacts.remove_in_iff.
+  split. exact H2. exact H1.
+  injection H; intros; subst.
+  destruct H0.
+  destruct H0.
+  discriminate.
+Admitted.
+
+Lemma wf4_preservation : forall sigma obs sigma' obs',
+  wf4 sigma -> <<sigma; obs>> ===> <<sigma'; obs'>> -> wf4 sigma'.
+Proof.
+  destruct sigma; destruct sigma'.
+  unfold wf4 in *.
+  intros; injection H1; intros.
+  inversion H0. inversion H18.
+  - subst. case_eq (eqb p1 p2).
+    intros. apply cmp_to_eq in H3. subst.
+    assert (NatMap.find p2 (NatMap.add p2 (process_value e' l' q0) p)
+    = Some (process_value e' l' q0)).
+    apply NatMapFacts.add_eq_o; reflexivity.
+    rewrite -> H2 in H3.
+    injection H3; intros; subst.
+    apply (H m mu rho p p2 l0 q0 e E).
+    reflexivity.
+    exact H19.
+    intros; apply cmp_to_uneq in H3.
+    assert (NatMap.find p1 (NatMap.add p2 (process_value e' l' q0) p) = NatMap.find p1 p).
+    apply NatMapFacts.add_neq_o; apply not_eq_sym; exact H3.
+    apply (H m mu rho p p1 l q e E).
+    reflexivity.
+    rewrite <- H4. exact H2.
+  - subst. case_eq (eqb p1 p2).
+    intros. apply cmp_to_eq in H3. subst.
+    assert (NatMap.find p2 (NatMap.add p2 (process_value e' l' q0) p)
+    = Some (process_value e' l' q0)).
+    apply NatMapFacts.add_eq_o; reflexivity.
+    rewrite -> H2 in H3.
+    injection H3; intros; subst.
+    destruct e0.
+    assert (e0 = enclave_ID_inactive \/ (exists raw_e : raw_enclave_ID,
+    e0 = enclave_ID_active raw_e /\ NatMap.In raw_e e1)).
+    apply (H m mu rho p p2 l0 q0 e0 e1).
+    reflexivity.
+    exact H19.
+    apply (wf4_enclave_creation e0 e1 e E mu n r_val2_addr r_val3).
+    exact H39.
+    exact H4.
+    intros; apply cmp_to_uneq in H3.
+    assert (NatMap.find p1 (NatMap.add p2 (process_value e' l' q0) p) = NatMap.find p1 p).
+    apply NatMapFacts.add_neq_o; apply not_eq_sym; exact H3.
+    apply (H m mu rho p p1 l q e E).
+    reflexivity.
+    rewrite <- H4. exact H2.
+  - subst. case_eq (eqb p1 p2).
+    intros. apply cmp_to_eq in H3. subst.
+    assert (NatMap.find p2 (NatMap.add p2 (process_value e' l' q0) p)
+    = Some (process_value e' l' q0)).
+    apply NatMapFacts.add_eq_o; reflexivity.
+    rewrite -> H2 in H3.
+    injection H3; intros; subst.
+    apply (H m m0 rho p p2 l0 q0 e E).
+    reflexivity.
+    exact H19.
+    intros; apply cmp_to_uneq in H3.
+    assert (NatMap.find p1 (NatMap.add p2 (process_value e' l' q0) p) = NatMap.find p1 p).
+    apply NatMapFacts.add_neq_o; apply not_eq_sym; exact H3.
+    apply (H m m0 rho p p1 l q e E).
+    reflexivity.
+    rewrite <- H4. exact H2.
+  - subst. case_eq (eqb p1 p2).
+    intros. apply cmp_to_eq in H3. subst.
+    assert (NatMap.find p2 (NatMap.add p2 (process_value (enclave_elimination (enclave_state_value
+    (enclave_ID_active e_raw) mem) r_val) l' q0) p) = Some (process_value (enclave_elimination
+    (enclave_state_value (enclave_ID_active e_raw) mem) r_val) l' q0)).
+    apply NatMapFacts.add_eq_o; reflexivity.
+    rewrite -> H2 in H3.
+    injection H3; intros; subst.
+    right.
+    (* issue with enclave elimination definition *)
+    give_up.
+    intros; apply cmp_to_uneq in H3.
+    assert (NatMap.find p1 (NatMap.add p2 (process_value (enclave_elimination (enclave_state_value
+    (enclave_ID_active e_raw) mem) r_val) l' q0) p) = NatMap.find p1 p).
+    apply NatMapFacts.add_neq_o; apply not_eq_sym; exact H3.
+    apply (H m m0 rho p p1 l q e E).
+    reflexivity.
+    rewrite <- H4. exact H2.
+  - subst. case_eq (eqb p1 p2).
+    intros. apply cmp_to_eq in H3. subst.
+    assert (NatMap.find p2 (NatMap.add p2 (process_value e' l' q0) p)
+    = Some (process_value e' l' q0)).
+    apply NatMapFacts.add_eq_o; reflexivity.
+    rewrite -> H2 in H3.
+    injection H3; intros; subst.
+    destruct e0.
+    assert (e0 = enclave_ID_inactive \/ (exists raw_e : raw_enclave_ID,
+    e0 = enclave_ID_active raw_e /\ NatMap.In raw_e e1)).
+    apply (H k mu rho p p2 l0 q0 e0 e1).
+    reflexivity.
+    exact H19.
+    apply (wf4_active_enclave_update e0 e1 e E (enclave_ID_active r_val)).
+    exact H35.
+    exact H4.
+    intros; apply cmp_to_uneq in H3.
+    assert (NatMap.find p1 (NatMap.add p2 (process_value e' l' q0) p) = NatMap.find p1 p).
+    apply NatMapFacts.add_neq_o; apply not_eq_sym; exact H3.
+    apply (H k mu rho p p1 l q e E).
+    reflexivity.
+    rewrite <- H4. exact H2.
+  - subst. case_eq (eqb p1 p2).
+    intros. apply cmp_to_eq in H3. subst.
+    assert (NatMap.find p2 (NatMap.add p2 (process_value e' l' q0) p)
+    = Some (process_value e' l' q0)).
+    apply NatMapFacts.add_eq_o; reflexivity.
+    rewrite -> H2 in H3.
+    injection H3; intros; subst.
+    destruct e0.
+    assert (e0 = enclave_ID_inactive \/ (exists raw_e : raw_enclave_ID,
+    e0 = enclave_ID_active raw_e /\ NatMap.In raw_e e1)).
+    apply (H k mu rho p p2 l0 q0 e0 e1).
+    reflexivity.
+    exact H19.
+    apply (wf4_active_enclave_update e0 e1 e E enclave_ID_inactive).
+    exact H34.
+    exact H4.
+    intros; apply cmp_to_uneq in H3.
+    assert (NatMap.find p1 (NatMap.add p2 (process_value e' l' q0) p) = NatMap.find p1 p).
+    apply NatMapFacts.add_neq_o; apply not_eq_sym; exact H3.
+    apply (H k mu rho p p1 l q e E).
+    reflexivity.
+    rewrite <- H4. exact H2.
+  - subst. case_eq (eqb p1 p2).
+    intros. apply cmp_to_eq in H3. subst.
+    assert (NatMap.find p2 (NatMap.add p2 (process_value e' l' q0) p)
+    = Some (process_value e' l' q0)).
+    apply NatMapFacts.add_eq_o; reflexivity.
+    rewrite -> H2 in H3.
+    injection H3; intros; subst.
+    apply (H k mu rho p p2 l0 q0 e E).
+    reflexivity.
+    exact H19.
+    intros; apply cmp_to_uneq in H3.
+    assert (NatMap.find p1 (NatMap.add p2 (process_value e' l' q0) p) = NatMap.find p1 p).
+    apply NatMapFacts.add_neq_o; apply not_eq_sym; exact H3.
+    apply (H k mu rho p p1 l q e E).
+    reflexivity.
+    rewrite <- H4. exact H2.
+  - subst. case_eq (eqb p1 p2).
+    intros. apply cmp_to_eq in H3. subst.
+    assert (NatMap.find p2 (NatMap.add p2 (process_value e' l' q0) p)
+    = Some (process_value e' l' q0)).
+    apply NatMapFacts.add_eq_o; reflexivity.
+    rewrite -> H2 in H3.
+    injection H3; intros; subst.
+    apply (H k mu rho p p2 l0 q0 e E).
+    reflexivity.
+    exact H19.
+    intros; apply cmp_to_uneq in H3.
+    assert (NatMap.find p1 (NatMap.add p2 (process_value e' l' q0) p) = NatMap.find p1 p).
+    apply NatMapFacts.add_neq_o; apply not_eq_sym; exact H3.
+    apply (H k mu rho p p1 l q e E).
+    reflexivity.
+    rewrite <- H4. exact H2.
+  - subst. case_eq (eqb p1 p2).
+    intros. apply cmp_to_eq in H3. subst.
+    assert (NatMap.find p2 (NatMap.add p2 (process_value e0 l0 q') p)
+    = Some (process_value e0 l0 q')).
+    apply NatMapFacts.add_eq_o; reflexivity.
+    rewrite -> H2 in H3.
+    injection H3; intros; subst.
+    apply (H k mu rho p p2 l0 q0 e E).
+    reflexivity.
+    exact H9.
+    intros; apply cmp_to_uneq in H3.
+    assert (NatMap.find p1 (NatMap.add p2 (process_value e0 l0 q') p) = NatMap.find p1 p).
+    apply NatMapFacts.add_neq_o; apply not_eq_sym; exact H3.
+    apply (H k mu rho p p1 l q e E).
+    reflexivity.
+    rewrite <- H4. exact H2.
+Admitted.
+
+Definition wf5 (sigma: runtime_state): Prop :=
+  forall k mu rho pi index F V C R p l q e E,
+  (sigma = runtime_state_value k mu rho pi) ->
+  (NatMap.find index k = Some (single_level_cache F V C R)) ->
+  (NatMap.find p pi = Some (process_value (enclave_state_value (enclave_ID_active e) E) l q)) ->
+  (NatMap.In e V).
+
+Lemma wf5_preservation : forall sigma obs sigma' obs',
+  wf5 sigma -> <<sigma; obs>> ===> <<sigma'; obs'>> -> wf5 sigma'.
+Proof.
+  destruct sigma; destruct sigma'.
+  unfold wf5 in *.
+  intros; injection H1; intros.
+  inversion H0. inversion H19.
+  - subst. give_up.
+  - subst. give_up.
+  - subst. give_up.
+  - subst. give_up.
+  - subst. give_up.
+  - subst. give_up.
+  - subst. give_up.
+  - subst. give_up.
+  - subst. give_up.
+Admitted.
